@prefix : <http://example.com/odp#> .
@prefix rdf: <http://www.w3.org/1999/02/22-rdf-syntax-ns#> .
@prefix rdfs: <http://www.w3.org/2000/01/rdf-schema#> .
@prefix owl: <http://www.w3.org/2002/07/owl#> .
@prefix skos: <http://www.w3.org/2004/02/skos/core#> .
@prefix schema: <http://schema.org/> .

: a owl:Ontology ;
    rdfs:comment "Ontology Design Pattern for Scientific Analysis Experiments" ;
    rdfs:label "ScientificAnalysisExperimentsODP" .

:Experiment a owl:Class ;
    rdfs:label "Experiment" ;
    skos:definition "A process or investigation intended to achieve a particular result."@en .

:SynthesisExperiment a owl:Class ;
    rdfs:label "Synthesis Experiment" ;
    skos:definition "A type of experiment intended to synthesize a sample."@en ;
    rdfs:subClassOf :Experiment .

:CharacterizationExperiment a owl:Class ;
    rdfs:label "Characterization Experiment" ;
    skos:definition "A type of experiment intended to characterize a sample."@en ;
    rdfs:subClassOf :Experiment .

:Role a owl:Class ;
    rdfs:label "Role" ;
    skos:definition "The function or participation of an object in an experiment."@en .

:Procedure a owl:Class ;
    rdfs:label "Procedure" ;
    skos:definition "A directive information content entity that describes how to achieve an objective."@en .

:Instrument a owl:Class ;
    rdfs:label "Instrument" ;
    skos:definition "A material entity that is created to serve a specific role or purpose."@en .

:Sample a owl:Class ;
    rdfs:label "Sample" ;
    skos:definition "A material entity that is intended to be the subject of study or investigation."@en .

:Result a owl:Class ;
    rdfs:label "Result" ;
    skos:definition "An information content entity that represents the output of an investigation or study."@en .

:hasParticipant a owl:ObjectProperty ;
    rdfs:label "hasParticipant" ;
    schema:domainIncludes :Experiment ;
    schema:rangeIncludes :Role ;
    skos:definition "Links an Experiment to a Role."@en .

:followedBy a owl:ObjectProperty ;
    rdfs:label "followedBy" ;
    schema:domainIncludes :Experiment ;
    schema:rangeIncludes :Experiment ;
    skos:definition "Links one Experiment to a subsequent Experiment."@en .

:Equipment a owl:Class ;
    rdfs:label "Equipment" ;
    skos:definition "A superclass for equipment used in experiments, such as an Instrument."@en .

:Material a owl:Class ;
    rdfs:label "Material" ;
    skos:definition "A superclass for materials used in experiments, such as a Sample."@en .

:Reagent a owl:Class ;
    rdfs:label "Reagent" ;
    skos:definition "A substance added to a system to cause a chemical reaction."@en ;
    rdfs:subClassOf :Material .

:Solvent a owl:Class ;
    rdfs:label "Solvent" ;
    skos:definition "A substance capable of dissolving other substances."@en ;
    rdfs:subClassOf :Material .

:usesEquipment a owl:ObjectProperty ;
    rdfs:label "usesEquipment" ;
    schema:domainIncludes :Experiment ;
    schema:rangeIncludes :Equipment ;
    skos:definition "Links an Experiment to an Equipment it uses."@en .

:usesMaterial a owl:ObjectProperty ;
    rdfs:label "usesMaterial" ;
    schema:domainIncludes :Experiment ;
    schema:rangeIncludes :Material ;
    skos:definition "Links an Experiment to a Material it uses."@en .

